src/program_proof/tulip/paxos/prelude.v
@@ -2,6 +2,6 @@ From Perennial.program_proof Require Export grove_prelude.
 From Perennial.program_logic Require Export atomic. (* prefer the ncfupd atomics *)
 From Perennial.program_proof.rsm Require Export big_sep.
 From Perennial.program_proof.rsm.pure Require Export
-  extend fin_maps list misc nat sets word quorum.
+  extend fin_maps fin_sets list misc nat sets word quorum.
 From Perennial.program_proof.tulip.paxos Require Export
   base consistency inv res.
